trace-symexec/attack1_straight_line_code-modulo-add-sub.bpl
@@ -10,7 +10,6 @@ axiom TwoE255 == TwoE64 * TwoE64 * TwoE64 * TwoE16 * TwoE16 * TwoE16 *32768;
 const TwoE256 : int; 
 axiom TwoE256 == TwoE64 * TwoE64 * TwoE64 * TwoE64;
 
-
 function sum(m: [address] uint256) returns (uint256);
 axiom (forall m: [address] uint256, a:address, v:uint256 :: sum(m[a:=v]) == sum(m) - m[a] + v);
 axiom (forall m: [address] uint256 :: ((forall a:address :: 0<=m[a]) ==> (forall a:address :: m[a]<=sum(m))));    
@@ -18,7 +17,6 @@ axiom (forall m: [address] uint256 :: ((forall a:address :: 0<=m[a]) ==> (forall
 function evmadd(a,b:uint256) returns (uint256);
 axiom (forall a,b: uint256 :: a+b < TwoE256 && a+b>=0 ==> evmadd(a,b) == a+b);
 axiom (forall a,b: uint256 :: a+b >= TwoE256 && a+b>=0 ==> evmadd(a,b) == a+b-TwoE256);
-
 
 function evmsub(a,b:uint256) returns (uint256);
 axiom (forall a,b: uint256 :: a-b < TwoE256 && a-b>=0 ==> sub(a,b) == a-b);
