trace-symexec/expected_output_theorem1.bpl
@@ -1,0 +1,81 @@
+type address = int;
+type uint256 = int;
+var totalSupply: uint256;
+const TwoE16 : uint256;
+axiom TwoE16 == 65536; 
+const TwoE64 : uint256; 
+axiom TwoE64 == TwoE16 * TwoE16 * TwoE16 * TwoE16;
+const TwoE255 : uint256;
+axiom TwoE255 == TwoE64 * TwoE64 * TwoE64 * TwoE16 * TwoE16 * TwoE16 *32768;
+const TwoE256 : int; 
+axiom TwoE256 == TwoE64 * TwoE64 * TwoE64 * TwoE64;
+
+function evmadd(a,b:uint256) returns (uint256);
+axiom (forall a,b: uint256 :: a+b < TwoE256 && a+b>=0 ==> evmadd(a,b) == a+b);
+axiom (forall a,b: uint256 :: a+b >= TwoE256 && a+b>=0 ==> evmadd(a,b) == a+b-TwoE256);
+
+function evmsub(a,b:uint256) returns (uint256);
+axiom (forall a,b: uint256 :: a-b < TwoE256 && a-b>=0 ==> evmsub(a,b) == a-b);
+axiom (forall a,b: uint256 :: a-b < TwoE256 && a-b<0 ==> evmsub(a,b) == a-b+TwoE256);
+
+function evmand(a, b:uint256) returns (uint256);
+axiom (forall a,b: uint256 :: a+b < TwoE256 && a+b>=0 ==> evmand(a,b) == a+b);
+axiom (forall a,b: uint256 :: a+b >= TwoE256 && a+b>=0 ==> evmand(a,b) == a+b-TwoE256);
+
+function sum(m: [address] uint256) returns (uint256);
+axiom (forall m: [address] uint256, a:address, v:uint256 :: sum(m[a:=v]) == sum(m) - m[a] + v);
+axiom (forall m: [address] uint256 :: ((forall a:address :: 0<=m[a]) ==> (forall a:address :: m[a]<=sum(m))));    
+
+var balances: [address] uint256;
+
+procedure straightline_code ()
+modifies balances;
+{  
+    var msg.sender: address ;
+    var _from: address ;
+    var _to: address;
+    var _value: uint256;
+    var _fee: uint256;
+       
+	var tmp2: uint256;
+	var tmp3: uint256;
+	var tmp1: uint256;
+	var tmp5: uint256;
+	var tmp6: uint256;
+	var tmp4: uint256;
+	var tmp7: bool;
+	var tmp8: bool;
+	var tmp9: bool;
+
+	assume(totalSupply<TwoE256 && msg.sender!=_to );
+	assume(forall x:address :: 0 <= balances[x] && balances[x] <= totalSupply);
+	assume( sum(balances) == totalSupply );
+
+	tmp2:=evmand(fff,msg.sender);
+	tmp3:=evmand(fff,_to);
+	tmp1:=evmsub(tmp2,tmp3);
+	assume(tmp1);
+
+	tmp5:=balances[_to];
+	tmp6:=balances[msg.sender];
+	tmp4:=evmadd(tmp5,tmp6);
+	balances[_to]:=tmp4;
+
+	tmp7:=!tmp6;
+	assume(tmp7);
+
+	tmp8:=!tmp7;
+	assume(tmp8);
+
+	tmp9:=!tmp8;
+	assume(tmp9);
+
+	assume(EQ(RETURNDATASIZE,0));
+
+	assume(GAS);
+
+	balances[msg.sender]:=0;
+
+	assert(forall x:address :: 0 <= balances[x] && balances[x] <= totalSupply);
+	assert( sum(balances) == totalSupply );
+}
